proof/agp32CorrectScript.sml
@@ -18,7 +18,8 @@ Proof
   rw [Init_def,Rel_def,is_sch_init_def] >>
   fs [agp32_init_IF_PC_input,agp32_init_EX_opc,IF_PC_Rel_def,IF_instr_Rel_def,
       Inv_Rel_def,enable_stg_def,EX_Rel_spec_def,isJump_isa_op_def,isJump_hw_op_def] >> fs [] >>
-  rw [agp32_init_ID_opc,agp32_init_EX_opc,agp32_init_EX_write_reg,agp32_init_EX_jump_sel,
+  rw [agp32_init_ID_opc,agp32_init_ID_addr_disable,
+      agp32_init_EX_opc,agp32_init_EX_write_reg,agp32_init_EX_jump_sel,
       agp32_init_MEM_opc,agp32_init_MEM_write_reg,agp32_init_WB_opc,
       agp32_init_WB_write_reg,agp32_init_WB_isOut] >>
   `a.data_in = (FUNPOW Next 0 a).data_in` by rw [] >>
